type check the remaining load and store instructions

Picinae_armv7.v
@@ -702,6 +702,17 @@ Definition arm_dec_bin_opt (n:N) :=
   else if ((xbits n 23 28) =? 1) && ((xbits n 4 8) =? 9) then
     ARM7_Mull (xbits n 28 32) (b 22 n) (b 21 n) (b 20 n) (xbits n 16 20) (xbits n 12 16) (xbits n 8 12) (xbits n 0 4)
 
+  else if (((xbits 25 28 n) =? 0) && ((xbits 22 21 n) =? 0) && ((xbits 7 12 n) =? 1) && ((xbits 4 5 n) =? 1)) then
+    (* Single data swap *)
+    match (b 6 n), (b 5 n), (b 20 n) with
+    | 0, 0, 0 => ARM7_Swp (xbits n 28 32) (xbits n 22 23) (xbits n 16 20) (xbits n 12 16) (xbits n 0 4)
+    (* Halfword data transfer: register offset *)
+    | _, _, 0 => ARM7_StrHS (xbits n 28 32) (xbits n 24 25) (xbits n 23 24) (xbits n 21 22)
+                            (xbits n 16 20) (xbits n 12 16) (xbits n 6 7) (xbits n 5 6) (xbits n 0 4)
+    | _, _, _ => ARM7_LdrHS (xbits n 28 32) (xbits n 24 25) (xbits n 23 24) (xbits n 21 22)
+                            (xbits n 16 20) (xbits n 12 16) (xbits n 6 7) (xbits n 5 6) (xbits n 0 4)
+    end
+
   (* Half word data transfer immediate offset *)
   else if (((xbits 25 28 n) =? 0) && ((xbits 22 21 n) =? 1) && ((xbits 7 8 n) =? 1) && ((xbits 4 5 n) =? 1)) then
     match (xbits n 20 21) with
@@ -710,22 +721,26 @@ Definition arm_dec_bin_opt (n:N) :=
     end (xbits n 28 32) (xbits n 24 25) (xbits n 23 24) (xbits n 21 22)
         (xbits n 16 20) (xbits n 12 16) (xbits n 6 7) (xbits n 5 6) (((xbits n 8 12) * 16) + (xbits n 0 4))
 
-  (* Halfword data transfer: register offset *)
-  else if (((xbits 25 28 n) =? 0) && ((xbits 22 21 n) =? 0) && ((xbits 7 12 n) =? 1) && ((xbits 4 5 n) =? 1)) then
-    match (b 6 n), (b 5 n), (b 20 n) with
-    | 0, 0, 0 => ARM7_Swp (xbits n 28 32) (xbits n 22 23) (xbits n 16 20) (xbits n 12 16) (xbits n 0 4)
+  (* Single data transfer register offset *)
+  else if ((xbits 25 28 n) =? 2) && ((xbits n 4 5) =? 0) then
+    match (xbits n 20 21) with
+    | 0 => ARM7_StrS
+    | _ => ARM7_LdrS
+    end (xbits n 28 32) (xbits n 24 25) (xbits n 23 24) (xbits n 22 23) (xbits n 21 22)
+        (xbits n 16 20) (xbits n 12 16) (xbits n 7 12) (xbits n 5 7) (xbits n 0 4)
 
-    | _, _, 0 => ARM7_StrHS (xbits n 28 32) (xbits n 24 25) (xbits n 23 24) (xbits n 21 22)
-                            (xbits n 16 20) (xbits n 12 16) (xbits n 6 7) (xbits n 5 6) (xbits n 0 4)
-    | _, _, _ => ARM7_LdrHS (xbits n 28 32) (xbits n 24 25) (xbits n 23 24) (xbits n 21 22)
-                            (xbits n 16 20) (xbits n 12 16) (xbits n 6 7) (xbits n 5 6) (xbits n 0 4)
-    end
+  (* Single data transfer immediate offset *)
+  else if ((xbits 25 28 n) =? 3) then
+    match (xbits n 20 21) with
+    | 0 => ARM7_StrI
+    | _ => ARM7_LdrI
+    end (xbits n 28 32) (xbits n 24 25) (xbits n 23 24) (xbits n 22 23) (xbits n 21 22)
+        (xbits n 16 20) (xbits n 12 16) (xbits n 0 12)
 
   (* Branch *)
   else if (xbits n 24 27) =? 5 then
     ARM7_Branch (xbits n 27 31) (xbits n 24 25) (toZ 24 (xbits n 0 24))
   else
-
     ARM7_Unsupported.
 
 Definition arm_dec_bin (n:N) :=
@@ -933,7 +948,7 @@ end.
 Open Scope stmt_scope.
 
 Definition arm7_st st := match st with | 0 => OP_LSHIFT | 1 => OP_RSHIFT | 2 => OP_ARSHIFT | _ => OP_ROT end.
-Definition ldr_str_word_bit b := match b with | 0 => 4 | _ => 1 end.
+Definition ldr_str_word_bit b := match b with | 0 => 32 | _ => 8 end.
 Definition ldr_str_up_bit u := match u with | 0 => OP_MINUS | _ => OP_PLUS end.
 Definition ldr_str_half_word_bit h := match h with | 0 => 8 | _ => 16 end.
 Definition ldr_str_signed_bit s := match s with | 0 => CAST_UNSIGNED | _ => CAST_SIGNED end.
@@ -1020,31 +1035,43 @@ Definition arm2il (ad:addr) armi :=
       cond_eval cond (
       match p with
       | 1 => Move (arm7_varid rd) (Load (Var V_MEM32)
-                                        (BinOp (ldr_str_up_bit u) (Var (arm7_varid rn)) (Word 32 imm))
+                                        (Cast CAST_SIGNED 32
+                                          (Cast CAST_LOW (ldr_str_word_bit b)
+                                            (BinOp (ldr_str_up_bit u) (Var (arm7_varid rn)) (Word imm 32))))
                                         LittleE
-                                        (ldr_str_word_bit b))
+                                        4)
       | _ => Move (arm7_varid rd) (Load (Var V_MEM32)
-                                        (Word 32 imm)
+                                        (Cast CAST_SIGNED 32
+                                            (Cast CAST_LOW (ldr_str_word_bit b)
+                                            (BinOp (ldr_str_up_bit u) (Var (arm7_varid rn)) (Word 0 32))))
                                         LittleE
-                                        (ldr_str_word_bit b))
+                                        4)
       end $;
       match w with
       | 0 => Nop
-      | _ => Move (arm7_varid rn) (BinOp (ldr_str_up_bit u) (Var (arm7_varid rn)) (Word 32 imm))
-      end)
+      | _ => Move (arm7_varid rn) (BinOp (ldr_str_up_bit u) (Var (arm7_varid rn)) (Word imm 32))
+      end) 
   | ARM7_StrI cond p u b w rn rd imm =>
       cond_eval cond (
       match p with
       | 1 => Move V_MEM32 (Store (Var V_MEM32)
-                          (BinOp (ldr_str_up_bit u) (Var (arm7_varid rn)) (Word 32 imm))
+                          (Cast CAST_SIGNED 32
+                            (Cast CAST_LOW (ldr_str_word_bit b)
+                              (BinOp (ldr_str_up_bit u) (Var (arm7_varid rn)) (Word imm 32))))
                           (Var (arm7_varid rd))
                           LittleE
-                          (ldr_str_word_bit b))
-      | _ => Move (arm7_varid rd) (Load (Var V_MEM32) (Word 32 imm) LittleE (ldr_str_word_bit b))
+                          4)
+      | _ => Move V_MEM32 (Store (Var V_MEM32)
+                          (Cast CAST_SIGNED 32
+                            (Cast CAST_LOW (ldr_str_word_bit b)
+                              (BinOp (ldr_str_up_bit u) (Var (arm7_varid rn)) (Word 0 32))))
+                          (Var (arm7_varid rd))
+                          LittleE
+                          4)
       end $;
       match w with
       | 0 => Nop
-      | _ => Move (arm7_varid rn) (BinOp (ldr_str_up_bit u) (Var (arm7_varid rn)) (Word 32 imm))
+      | _ => Move (arm7_varid rn) (BinOp (ldr_str_up_bit u) (Var (arm7_varid rn)) (Word imm 32))
       end)
   | ARM7_LdrS cond p u b w rn rd sa st rm =>
       cond_eval cond (
@@ -1052,18 +1079,22 @@ Definition arm2il (ad:addr) armi :=
       | 1 =>
         Move (arm7_varid rd)
              (Load (Var V_MEM32)
-                   (BinOp (ldr_str_up_bit u)
-                          (Var (arm7_varid rn))
-                          (BinOp (arm7_st st) (Var (arm7_varid rm)) (Word 32 sa)))
+                   (Cast CAST_SIGNED 32
+                      (Cast CAST_LOW (ldr_str_word_bit b)
+                          (BinOp (ldr_str_up_bit u)
+                              (Var (arm7_varid rn))
+                              (BinOp (arm7_st st) (Var (arm7_varid rm)) (Word sa 32)))))
                    LittleE
-                   (ldr_str_word_bit b)
+                   4
              )
       | _ =>
         Move (arm7_varid rd)
              (Load (Var V_MEM32)
-                   (BinOp (arm7_st st) (Var (arm7_varid rm)) (Word 32 sa))
+                   (Cast CAST_SIGNED 32
+                      (Cast CAST_LOW (ldr_str_word_bit b)
+                          (BinOp (arm7_st st) (Var (arm7_varid rm)) (Word sa 32))))
                    LittleE
-                   (ldr_str_word_bit b)
+                   4
              )
       end $;
       match w with
@@ -1071,30 +1102,34 @@ Definition arm2il (ad:addr) armi :=
       | _ => Move (arm7_varid rn)
                   (BinOp (ldr_str_up_bit u)
                          (Var (arm7_varid rn))
-                         (BinOp (arm7_st st) (Var (arm7_varid rm)) (Word 32 sa)))
+                         (BinOp (arm7_st st) (Var (arm7_varid rm)) (Word sa 32)))
       end)
   | ARM7_StrS cond p u b w rn rd sa st rm =>
       cond_eval cond (
       match p with
       | 1 => Move V_MEM32 (Store (Var V_MEM32)
-                                 (BinOp (ldr_str_up_bit u)
-                                        (Var (arm7_varid rn))
-                                        (BinOp (arm7_st st) (Var (arm7_varid rm)) (Word 32 sa)))
+                                 (Cast CAST_SIGNED 32
+                                    (Cast CAST_LOW (ldr_str_word_bit b)
+                                        (BinOp (ldr_str_up_bit u)
+                                            (Var (arm7_varid rn))
+                                            (BinOp (arm7_st st) (Var (arm7_varid rm)) (Word sa 32)))))
                                  (Var (arm7_varid rd))
                                  LittleE
-                                 (ldr_str_word_bit b))
-      | _ => Move (arm7_varid rd)
-                  (Load (Var V_MEM32)
-                        (BinOp (arm7_st st) (Var (arm7_varid rm)) (Word 32 sa))
-                        LittleE
-                        (ldr_str_word_bit b))
+                                 4)
+      | _ => Move V_MEM32 (Store (Var V_MEM32)
+                                 (Cast CAST_SIGNED 32
+                                    (Cast CAST_LOW (ldr_str_word_bit b)
+                                      (Var (arm7_varid rn))))
+                                 (Var (arm7_varid rd))
+                                 LittleE
+                                 4)
       end $;
       match w with
       | 0 => Nop
       | _ => Move (arm7_varid rn)
                   (BinOp (ldr_str_up_bit u)
                          (Var (arm7_varid rn))
-                         (BinOp (arm7_st st) (Var (arm7_varid rm)) (Word 32 sa)))
+                         (BinOp (arm7_st st) (Var (arm7_varid rm)) (Word sa 32)))
       end)
   | ARM7_LdrHS cond p u w rn rd s h rm =>
       cond_eval cond (
@@ -1307,6 +1342,7 @@ Proof.
               try unfold ldr_str_signed_bit;
               try unfold ldr_str_half_word_bit;
               try unfold ldr_str_up_bit;
+              try unfold ldr_str_word_bit;
               try unfold arm7_st.
   all: repeat match goal with |- context [ match ?x with _ => _ end ] =>
     try destruct x
